Prove coordinator recovery at the protocol level
Add the following resources:
1. [txn_client_token] used to prove rank-freshness for client slow-path
2. [replica_backup_vote] and [replica_backup_token] used to prove rank-freshness
for backup coordinators

Add rank-freshness invariants to replica

Prove invariance w.r.t.
1. advance
2. accept
3. propose

Update linearize to give [txn_client_token]

src/program_proof/tulip/cmd.v
@@ -374,14 +374,14 @@ Section execute_cmds.
   | LocalState
       (cm : gmap nat bool) (hists : gmap dbkey dbhist) (cpm : gmap nat dbmap)
       (ptgsm : gmap nat (gset u64)) (sptsm ptsm : gmap dbkey nat)
-      (bm : gmap nat ballot) (ladm : gmap nat nat)
+      (bm : gmap nat ballot) (laim : gmap nat nat)
   | LocalStuck.
 
   Definition not_local_stuck st := st ≠ LocalStuck.
 
   Definition execute_commit st (tid : nat) (pwrs : dbmap) :=
     match st with
-    | LocalState cm hists cpm ptgsm sptsm ptsm bm ladm =>
+    | LocalState cm hists cpm ptgsm sptsm ptsm bm laim =>
         match cm !! tid with
         | Some true => st
         | Some false => LocalStuck
@@ -389,10 +389,10 @@ Section execute_cmds.
                  | Some _ => LocalState
                               (<[tid := true]> cm) (multiwrite tid pwrs hists)
                               (delete tid cpm) (delete tid ptgsm) sptsm (release pwrs ptsm)
-                              bm ladm
+                              bm laim
                  | None => LocalState
                             (<[tid := true]> cm) (multiwrite tid pwrs hists)
-                            cpm ptgsm sptsm ptsm bm ladm
+                            cpm ptgsm sptsm ptsm bm laim
                  end
         end
     | LocalStuck => LocalStuck
@@ -400,15 +400,15 @@ Section execute_cmds.
 
   Definition execute_abort st (tid : nat) :=
     match st with
-    | LocalState cm hists cpm ptgsm sptsm ptsm bm ladm =>
+    | LocalState cm hists cpm ptgsm sptsm ptsm bm laim =>
         match cm !! tid with
         | Some true => LocalStuck
         | Some false => st
         | None => match cpm !! tid with
                  | Some pwrs => LocalState
                                  (<[tid := false]> cm) hists (delete tid cpm)
-                                 (delete tid ptgsm) sptsm (release pwrs ptsm) bm ladm
-                 | None => LocalState (<[tid := false]> cm) hists cpm ptgsm sptsm ptsm bm ladm
+                                 (delete tid ptgsm) sptsm (release pwrs ptsm) bm laim
+                 | None => LocalState (<[tid := false]> cm) hists cpm ptgsm sptsm ptsm bm laim
                  end
         end
     | LocalStuck => LocalStuck
@@ -416,37 +416,45 @@ Section execute_cmds.
 
   Definition execute_acquire st (tid : nat) (pwrs : dbmap) (ptgs : gset u64) :=
     match st with
-    | LocalState cm hists cpm ptgsm sptsm ptsm bm ladm =>
+    | LocalState cm hists cpm ptgsm sptsm ptsm bm laim =>
         LocalState
           cm hists (<[tid := pwrs]> cpm) (<[tid := ptgs]> ptgsm)
-          (setts (S tid) pwrs sptsm) (acquire tid pwrs ptsm) bm ladm
+          (setts (S tid) pwrs sptsm) (acquire tid pwrs ptsm) bm laim
     | LocalStuck => LocalStuck
     end.
 
   Definition execute_read st (tid : nat) (key : dbkey) :=
     match st with
-    | LocalState cm hists cpm ptgsm sptsm ptsm bm ladm =>
+    | LocalState cm hists cpm ptgsm sptsm ptsm bm laim =>
         LocalState
-          cm hists cpm ptgsm (alter (λ spts, (spts `max` tid)%nat) key sptsm) ptsm bm ladm
+          cm hists cpm ptgsm (alter (λ spts, (spts `max` tid)%nat) key sptsm) ptsm bm laim
     | LocalStuck => LocalStuck
     end.
 
   Definition execute_advance st (tid : nat) (rank : nat) :=
     match st with
-    | LocalState cm hists cpm ptgsm sptsm ptsm bm ladm =>
-        LocalState
-          cm hists cpm ptgsm sptsm ptsm
-          (alter (λ l, extend tid Reject l) tid bm) ladm
+    | LocalState cm hists cpm ptgsm sptsm ptsm bm laim =>
+        let blt := extend rank Reject (match bm !! tid with
+                                       | Some l => l
+                                       | None => [Accept false]
+                                       end) in
+        let laim' := match laim !! tid with
+                     | Some _ => laim
+                     | _ => <[tid := O]> laim
+                     end in
+        LocalState cm hists cpm ptgsm sptsm ptsm (<[tid := blt]> bm) laim'
     | LocalStuck => LocalStuck
     end.
 
   Definition execute_accept st (tid : nat) (rank : nat) (pdec : bool) :=
     match st with
-    | LocalState cm hists cpm ptgsm sptsm ptsm bm ladm =>
+    | LocalState cm hists cpm ptgsm sptsm ptsm bm laim =>
+        let blt := match bm !! tid with
+                   | Some l => extend rank Reject l
+                   | None => replicate rank Reject
+                   end ++ [Accept pdec] in
         LocalState
-          cm hists cpm ptgsm sptsm ptsm
-          (alter (λ l, extend tid Reject l ++ [Accept pdec]) tid bm)
-          (<[tid := rank]> ladm)
+          cm hists cpm ptgsm sptsm ptsm (<[tid := blt]> bm) (<[tid := rank]> laim)
     | LocalStuck => LocalStuck
     end.
 
@@ -476,14 +484,14 @@ Section execute_cmds.
     execute_cmds (cmds ++ [cmd]) = execute_cmd (execute_cmds cmds) cmd.
   Proof. by rewrite /execute_cmds foldl_snoc. Qed.
 
-  Lemma execute_cmds_dom_histm {log cm histm cpm ptgsm sptsm ptsm bm ladm} :
-    execute_cmds log = LocalState cm histm cpm ptgsm sptsm ptsm bm ladm ->
+  Lemma execute_cmds_dom_histm {log cm histm cpm ptgsm sptsm ptsm bm laim} :
+    execute_cmds log = LocalState cm histm cpm ptgsm sptsm ptsm bm laim ->
     dom histm = keys_all.
   Proof.
   Admitted.
 
-  Lemma execute_cmds_hist_not_nil {log cm histm cpm ptgsm sptsm ptsm bm ladm} :
-    execute_cmds log = LocalState cm histm cpm ptgsm sptsm ptsm bm ladm ->
+  Lemma execute_cmds_hist_not_nil {log cm histm cpm ptgsm sptsm ptsm bm laim} :
+    execute_cmds log = LocalState cm histm cpm ptgsm sptsm ptsm bm laim ->
     map_Forall (λ _ h, h ≠ []) histm.
   Admitted.
 
@@ -507,8 +515,8 @@ Section merge_clog_ilog.
 
   Lemma execute_cmds_apply_cmds clog ilog cm histm :
     let log := merge_clog_ilog clog ilog in
-    (∃ cpm ptgsm sptsm ptsm bm ladm,
-        execute_cmds log = LocalState cm histm cpm ptgsm sptsm ptsm bm ladm) ->
+    (∃ cpm ptgsm sptsm ptsm bm laim,
+        execute_cmds log = LocalState cm histm cpm ptgsm sptsm ptsm bm laim) ->
     apply_cmds clog = State cm histm.
   Admitted.
 End merge_clog_ilog.
