src/program_proof/tulip/invariance/advance.v
@@ -1,0 +1,283 @@
+From Perennial.program_proof.tulip Require Import prelude.
+
+Lemma confined_by_ballot_map_inv_advance_absent
+  {A} (bm : gmap nat ballot) (mm : gmap nat (gmap nat A)) ts l r x :
+  bm !! ts = None ->
+  (r ≤ length l)%nat ->
+  confined_by_ballot_map bm mm ->
+  confined_by_ballot_map (<[ts := l]> bm) (<[ts := {[r := x]}]> mm).
+Proof.
+  intros Hnone Hlen Hbm.
+  apply map_Forall2_insert_2; last done.
+  intros rx Hrx.
+  rewrite lookup_insert_ne; first done.
+  clear -Hlen Hrx. lia.
+Qed.
+
+Lemma confined_by_ballot_map_inv_advance_present
+  {A} (bm : gmap nat ballot) (mm : gmap nat (gmap nat A)) ts l m r x :
+  mm !! ts = Some m ->
+  bm !! ts = Some l ->
+  confined_by_ballot_map bm mm ->
+  confined_by_ballot_map (<[ts := extend r Reject l]> bm) (<[ts := <[r := x]> m]> mm).
+Proof.
+  intros Hm Hl Hbm.
+  apply map_Forall2_insert_2; last done.
+  apply map_Forall2_forall in Hbm as [Hbm _].
+  specialize (Hbm _ _ _ Hl Hm).
+  intros rx Hrx.
+  rewrite extend_length in Hrx.
+  rewrite lookup_insert_ne; last lia.
+  apply Hbm.
+  lia.
+Qed.
+
+Definition advance_requirement st ts rk :=
+  match st with
+  | LocalState _ _ _ _ _ _ bm _ =>
+      match bm !! ts with
+      | Some l => (length l < rk)%nat
+      | _ => (O < rk)%nat
+      end
+  | _ => False
+  end.
+
+Definition last_accepted_decision st ts p :=
+  match st with
+  | LocalState _ _ _ _ _ _ bm laim =>
+      match bm !! ts, laim !! ts with
+      | Some l, Some i => l !! i = Some (Accept p)
+      | Some _, None => False
+      | None, Some _ => False
+      | None, None => p = false
+      end
+  | _ => False
+  end.
+
+Section advance.
+  Context `{!tulip_ghostG Σ}.
+
+  (* TODO: When this lemma is used for becoming the coordinator, [cid = (gid,
+  rid)]. For use when receiving an inquire message, still need to figure out how
+  [cid] is obtained. Worst case is to include them physically in the message. *)
+
+  Lemma replica_inv_advance γ gid rid clog ilog st ts rk cid :
+    execute_cmds (merge_clog_ilog clog ilog) = st ->
+    advance_requirement st ts rk ->
+    own_replica_clog_half γ rid clog -∗
+    own_replica_ilog_half γ rid ilog -∗
+    replica_inv γ gid rid ==∗
+    own_replica_clog_half γ rid clog ∗
+    own_replica_ilog_half γ rid (ilog ++ [(length clog, CmdAdvance ts rk)]) ∗
+    replica_inv γ gid rid ∗
+    ([∗ set] tgid ∈ gids_all, own_replica_backup_token γ gid rid ts rk tgid) ∗
+    is_replica_backup_vote γ gid rid ts rk cid ∗
+    ∃ p, prepare_promise γ gid rid ts rk p ∗
+         ⌜last_accepted_decision st ts p⌝.
+  Proof.
+    iIntros (Hst Hrequire) "Hclogprog Hilogprog Hrp".
+    do 2 iNamed "Hrp".
+    (* Agreement on the consistent and inconsistent logs. *)
+    iDestruct (replica_clog_agree with "Hclogprog Hclog") as %->.
+    iDestruct (replica_ilog_agree with "Hilogprog Hilog") as %->.
+    (* Update the inconsistent log. *)
+    set ilog' := ilog ++ _.
+    iMod (replica_ilog_update ilog' with "Hilogprog Hilog") as "[Hilogprog Hilog]".
+    set st' := execute_advance st ts rk.
+    (* This will evaluate to the right form to re-establish the RSM invariant. *)
+    assert (Hrsm' : execute_cmds (merge_clog_ilog clog ilog') = st').
+    { rewrite merge_clog_ilog_snoc_ilog; last done.
+      by rewrite execute_cmds_snoc Hst /=.
+    }
+    destruct st as [cmx histmx cpmx ptgsmx sptsmx ptsmx bmx laimx |]; last done.
+    simpl in Hrequire.
+    rewrite Hrsm in Hst. symmetry in Hst. inv Hst.
+    iNamed "Hbackup".
+    iNamed "Hbm".
+    simpl in Hrsm'.
+    destruct (bm !! ts) as [blt |] eqn:Hbmts; last first.
+    { (* Case: [bm !! ts = None]. *)
+      set blt' := extend _ _ _ in Hrsm'.
+      (* Insert [(ts, blt')] into the ballot map. *)
+      iMod (replica_ballot_insert ts blt' with "Hblt") as "Hbm".
+      { apply Hbmts. }
+      set bm' := insert _ _ bm.
+      (* Extract a witness that this replica accepts [false] at the fast rank. *)
+      iAssert (prepare_promise γ gid rid ts rk false)%I as "#Hpromise".
+      { iDestruct (replica_ballot_witness ts with "Hbm") as "#Hlb".
+        { by rewrite lookup_insert. }
+        iFrame "Hlb".
+        subst blt'.
+        rewrite latest_term_extend_Reject latest_term_singleton.
+        iSplit; first done.
+        iPureIntro.
+        split.
+        { rewrite lookup_extend_l; first done. simpl. lia. }
+        { rewrite extend_length. simpl. clear -Hrequire. lia. }
+      }
+      (* Vote for [cid] by inserting [(rk, cid)] into the submap of bvm. *)
+      (* Insert [(ts, ∅)] into the backup vote map. *)
+      iMod (replica_backup_vote_init ts with "Hbvm") as "Hbvm".
+      { rewrite -not_elem_of_dom Hdombvm. by apply not_elem_of_dom in Hbmts. }
+      (* And then insert [(rk, cid)] into the submap. *)
+      iMod (replica_backup_vote_insert ts rk cid with "Hbvm") as "[Hbvm #Hvote]".
+      { by rewrite lookup_insert. }
+      { done. }
+      (* Obtain exclusive tokens for [cid] by inserting [(rk, cid)] into the submap of btm. *)
+      (* Insert [(ts, ∅)] into the backup token map. *)
+      iMod (replica_backup_token_init ts with "Hbtm") as "Hbtm".
+      { rewrite -not_elem_of_dom Hdombtm. by apply not_elem_of_dom in Hbmts. }
+      (* And then insert [(rk, gids_all)] into the submap. *)
+      iMod (replica_backup_token_insert ts rk gids_all with "Hbtm") as "[Hbtm Hbts]".
+      { by rewrite lookup_insert. }
+      { done. }
+      iAssert (replica_inv_backup γ gid rid bm')%I with "[$Hbvm $Hbtm]" as "Hbackup".
+      { iPureIntro.
+        rewrite 5!dom_insert_L Hdombvm Hdombtm.
+        do 2 (split; first set_solver).
+        rewrite 2!insert_empty 2!insert_insert.
+        split.
+        { apply confined_by_ballot_map_inv_advance_absent; [apply Hbmts | | apply Hbmbvm].
+          rewrite extend_length /=.
+          clear -Hrequire. lia.
+        }
+        { apply confined_by_ballot_map_inv_advance_absent; [apply Hbmts | | apply Hbmbtm].
+          rewrite extend_length /=.
+          clear -Hrequire. lia.
+        }
+      }
+      iFrame "Hclogprog Hilogprog Hbackup Hpromise Hvote Hbts".
+      iFrame "∗ # %".
+      iModIntro.
+      assert (laim !! ts = None) as Hlaimts.
+      { apply map_Forall2_dom_L in Hbmlaim.
+        by rewrite -not_elem_of_dom -Hbmlaim not_elem_of_dom.
+      }
+      iSplit; last first.
+      { iPureIntro.
+        by rewrite /= Hbmts Hlaimts.
+      }
+      iSplit.
+      { iApply (big_sepM_insert_2 with "[] Hsafebm").
+        subst blt'.
+        iIntros (r).
+        case_decide as Hr; first done.
+        destruct (decide (rk ≤ r)%nat) as [Hge | Hlt].
+        { rewrite lookup_ge_None_2; first done.
+          rewrite extend_length /=.
+          clear -Hr Hge. lia.
+        }
+        rewrite lookup_extend_r; first done.
+        simpl.
+        clear -Hr Hlt. lia.
+      }
+      iPureIntro.
+      rewrite Hlaimts.
+      apply map_Forall2_insert_2; last apply Hbmlaim.
+      rewrite latest_term_extend_Reject latest_term_singleton.
+      split; first done.
+      exists false.
+      rewrite lookup_extend_l; first done.
+      simpl. lia.
+    }
+    set blt' := extend _ _ _ in Hrsm'.
+    (* Insert [(ts, blt')] into the ballot map. *)
+    iMod (replica_ballot_update ts _ blt' with "Hblt") as "Hbm".
+    { apply Hbmts. }
+    { apply extend_prefix. }
+    set bm' := insert _ _ bm.
+    apply map_Forall2_forall in Hbmlaim as Hp.
+    destruct Hp as [Hp Hdomlaim].
+    assert (is_Some (laim !! ts)) as [i Hlaimts].
+    { by rewrite -elem_of_dom -Hdomlaim elem_of_dom. }
+    specialize (Hp _ _ _ Hbmts Hlaimts).
+    destruct Hp as [Hlatest [p Hp]].
+    subst i.
+    (* Extract a witness that this replica accepts [p] at the latest rank in [blt]. *)
+    iAssert (prepare_promise γ gid rid ts rk p)%I as "#Hpromise".
+    { iDestruct (replica_ballot_witness ts with "Hbm") as "#Hlb".
+      { by rewrite lookup_insert. }
+      iFrame "Hlb".
+      subst blt'.
+      rewrite latest_term_extend_Reject.
+      iSplit.
+      { rewrite /is_group_prepare_proposal_if_classic.
+        case_decide as Hnz; first done.
+        iDestruct (big_sepM_lookup with "Hsafebm") as "Hsafeblt"; first apply Hbmts.
+        iSpecialize ("Hsafeblt" $! (latest_term blt)).
+        case_decide as Hnz'; first done.
+        by rewrite Hp.
+      }
+      iPureIntro.
+      split.
+      { rewrite lookup_extend_l; first apply Hp.
+        apply latest_term_length_lt.
+        by intros ->.
+      }
+      { rewrite extend_length. clear -Hrequire. lia. }
+    }
+    (* Vote for [cid] by inserting [(rk, cid)] into the submap of bvm. *)
+    assert (is_Some (bvm !! ts)) as [bvmts Hbvmts].
+    { by rewrite -elem_of_dom Hdombvm elem_of_dom. }
+    iMod (replica_backup_vote_insert ts rk cid with "Hbvm") as "[Hbvm #Hvote]".
+    { apply Hbvmts. }
+    { apply map_Forall2_forall in Hbmbvm as [Hbmbvm _].
+      specialize (Hbmbvm _ _ _ Hbmts Hbvmts).
+      apply Hbmbvm, Hrequire.
+    }
+    (* Obtain exclusive tokens for [cid] by inserting [(rk, cid)] into the submap of btm. *)
+    assert (is_Some (btm !! ts)) as [btmts Hbtmts].
+    { by rewrite -elem_of_dom Hdombtm elem_of_dom. }
+    iMod (replica_backup_token_insert ts rk gids_all with "Hbtm") as "[Hbtm Hbts]".
+    { apply Hbtmts. }
+    { apply map_Forall2_forall in Hbmbtm as [Hbmbtm _].
+      specialize (Hbmbtm _ _ _ Hbmts Hbtmts).
+      apply Hbmbtm, Hrequire.
+    }
+    iAssert (replica_inv_backup γ gid rid bm')%I with "[$Hbvm $Hbtm]" as "Hbackup".
+    { iPureIntro.
+      rewrite 3!dom_insert_L Hdombvm Hdombtm.
+      do 2 (split; first done).
+      split; by eapply confined_by_ballot_map_inv_advance_present.
+    }
+    iFrame "Hclogprog Hilogprog Hbackup Hpromise Hvote Hbts".
+    iFrame "∗ # %".
+    iModIntro.
+    iSplit; last first.
+    { iPureIntro.
+      by rewrite /= Hbmts Hlaimts.
+    }
+    iSplit.
+    { iApply (big_sepM_insert_2 with "[] Hsafebm").
+      subst blt'.
+      iIntros (r).
+      case_decide as Hr; first done.
+      destruct (decide (rk ≤ r)%nat) as [Hge | Hlt].
+      { rewrite lookup_ge_None_2; first done.
+        rewrite extend_length /=.
+        clear -Hrequire Hge. lia.
+      }
+      destruct (decide (length blt ≤ r)%nat) as [Hgelen | Hltlen].
+      { rewrite lookup_extend_r; first done.
+        clear -Hgelen Hlt. lia.
+      }
+      rewrite lookup_extend_l; last first.
+      { clear -Hltlen. lia. }
+      iDestruct (big_sepM_lookup with "Hsafebm") as "Hsafeblt"; first apply Hbmts.
+      iSpecialize ("Hsafeblt" $! r).
+      by case_decide.
+    }
+    iPureIntro.
+    rewrite Hlaimts.
+    rewrite -(insert_id _ _ _ Hlaimts).
+    apply map_Forall2_insert_2; last apply Hbmlaim.
+    split.
+    { by rewrite latest_term_extend_Reject. }
+    { exists p.
+      rewrite lookup_extend_l; first done.
+      apply latest_term_length_lt.
+      by intros ->.
+    }
+  Qed.
+
+End advance.
