src/program_proof/tulip/invariance/propose.v
@@ -1,0 +1,72 @@
+From Perennial.program_proof.tulip Require Import prelude.
+
+Section propose.
+  Context `{!tulip_ghostG Σ}.
+
+  Lemma group_inv_propose γ gid ts rk p :
+    rk ≠ O ->
+    safe_proposal γ gid ts rk p -∗
+    exclusive_proposal γ gid ts rk -∗
+    group_inv γ gid ==∗
+    group_inv γ gid ∗
+    is_group_prepare_proposal γ gid ts rk p.
+  Proof.
+    iIntros (Hnz) "#Hsafepsl Hexcl Hgroup".
+    do 2 iNamed "Hgroup". iNamed "Hpsm".
+    destruct (psm !! ts) as [ps |] eqn:Hpsmts; last first.
+    { (* Case: [psm !! ts = None]. *)
+      iMod (group_prepare_proposal_init ts {[rk := p]} with "Hpsm") as "Hpsm".
+      { apply Hpsmts. }
+      iDestruct (group_prepare_proposal_witness ts _ rk p with "Hpsm") as "#Hpsl".
+      { by rewrite lookup_insert. }
+      { by rewrite lookup_singleton. }
+      iFrame "∗ # %".
+      iModIntro.
+      iSplit.
+      { iApply (big_sepM_insert_2 with "[Hexcl] Hfresh").
+        by rewrite /exclusive_proposals dom_singleton_L big_sepS_singleton.
+      }
+      iSplit.
+      { iApply big_sepM_insert_2; last done.
+        by rewrite /safe_proposals big_sepM_singleton.
+      }
+      iPureIntro.
+      by apply map_Forall_insert_2; first rewrite lookup_insert_ne.
+    }
+    (* Case: [psm !! ts = Some ps]. *)
+    (* Prove freshness of rank [rk] in [ps]. *)
+    destruct (ps !! rk) as [b |] eqn:Hfresh.
+    { iDestruct (big_sepM_lookup with "Hfresh") as "Hexcls"; first apply Hpsmts.
+      apply elem_of_dom_2 in Hfresh.
+      iDestruct (big_sepS_elem_of with "Hexcls") as "Hexcl'"; first apply Hfresh.
+      iDestruct (exclusive_proposal_excl with "Hexcl Hexcl'") as %[].
+    }
+    iMod (group_prepare_proposal_insert ts _ rk p with "Hpsm") as "Hpsm".
+    { apply Hpsmts. }
+    { apply Hfresh. }
+    iDestruct (group_prepare_proposal_witness ts _ rk p with "Hpsm") as "#Hpsl".
+    { by rewrite lookup_insert. }
+    { by rewrite lookup_insert. }
+    iFrame "∗ # %".
+    iModIntro.
+    iSplit.
+    { rewrite -insert_delete_insert.
+      iDestruct (big_sepM_delete with "Hfresh") as "[Hfreshts Hfresh]".
+      { apply Hpsmts. }
+      iApply (big_sepM_insert_2 with "[Hfreshts Hexcl] Hfresh").
+      rewrite /exclusive_proposals dom_insert_L.
+      iApply (big_sepS_insert_2 with "Hexcl Hfreshts").
+    }
+    iSplit.
+    { iApply big_sepM_insert_2; last done.
+      iDestruct (big_sepM_lookup with "Hsafepsm") as "Hsafeps".
+      { apply Hpsmts. }
+      by iApply big_sepM_insert_2.
+    }
+    iPureIntro.
+    apply map_Forall_insert_2; last done.
+    rewrite lookup_insert_ne; last done.
+    by specialize (Hzunused _ _ Hpsmts).
+  Qed.
+
+End propose.
